theories/NP/TM/LM_to_mTM.v
@@ -429,7 +429,7 @@ Smpl Add 1 eapply pTC_inl : polyTimeComputable.
 From Complexity.Complexity Require Import Subtypes.
 Import Datatypes.Lists Datatypes.LBool.
 Lemma LMGenNP_to_TMGenNP_mTM:
-  restrictBy (LMHaltsOrDiverges (list bool)) (LMGenNP (list bool)) ⪯p (restrictBy (HaltsOrDiverges_fixed_mTM (projT1 M.M)) (TMGenNP_fixed_mTM (projT1 M.M))).
+  LMGenNP (list bool) ⪯p (restrictBy (HaltsOrDiverges_fixed_mTM (projT1 M.M)) (TMGenNP_fixed_mTM (projT1 M.M))).
 Proof.
   evar (f__size:nat -> nat).
   enough (Hcert_f__size : forall maxSize (bs : list bool) sig R, size (enc bs) <= maxSize -> sizeOfTape (initValue (sig:=sig) _ R bs) <= f__size maxSize).
